Give up on trying to use arbitrary Coq values.
We now have a "type" type and a "value" type in ast.v. Type equality
is now decidable so the problems with existT can be retired. But now
there's another problem: you can't destruct boolean values...

src/ast.v
@@ -16,19 +16,35 @@ Import ListNotations.
  * abstract syntax the code is written in
  *)
 
-(* types go here *)
+(* types are the types of values we can touch directly *)
+Inductive type :=
+| t_unit: type
+| t_nat: type
+| t_bool: type
+| t_pair: type -> type -> type
+| t_list: type -> type
+| t_lock: type -> type
+.
 
 (* variables are identified with numbers *)
-Inductive var: Type -> Type :=
+Inductive var: type -> Type :=
 | mkvar: forall t, nat -> var t
 .
 
 (* locks are a special class of variables *)
-Inductive lock: Type -> Type :=
+Inductive lock: type -> Type :=
 | mklock : forall t, nat -> bool -> lock t
 .
 
-(* values go here *)
+Inductive value: type -> Type :=
+| v_unit: value t_unit
+| v_nat (n: nat): value t_nat
+| v_bool (b: bool): value t_bool
+| v_pair (ta: type) (a: value ta) (tb: type) (b: value tb):
+     value (t_pair ta tb)
+| v_list (t: type) (l: list (value t)): value (t_list t)
+| v_lock (t: type) (l: lock t): value (t_lock t)
+.
 
 Inductive invariant : Type :=
 (* Just an example *)
@@ -38,10 +54,10 @@ Inductive invariant : Type :=
 (*
  * expressions produce values
  *)
-Inductive expr: Type -> Type :=
-| e_value: forall (t : Type), t -> expr t
-| e_read: forall (t: Type), var t -> expr t
-| e_cond: forall t, expr bool -> expr t -> expr t -> expr t
+Inductive expr: type -> Type :=
+| e_value: forall (t : type), value t -> expr t
+| e_read: forall (t: type), var t -> expr t
+| e_cond: forall t, expr t_bool -> expr t -> expr t -> expr t
 .
 
 (*
@@ -49,14 +65,14 @@ Inductive expr: Type -> Type :=
  *)
 Inductive stmt: Type :=
 | s_block: list stmt -> stmt
-| s_start: forall (pt : Type), proc pt unit -> expr pt -> stmt
+| s_start: forall (pt : type), proc pt t_unit -> expr pt -> stmt
 | s_assign: forall t, var t -> expr t -> stmt
 | s_load: forall t, var t -> lock t -> stmt
 | s_store: forall t, lock t -> expr t -> stmt
 | s_scope: stmt -> stmt
-| s_if: expr bool -> stmt -> stmt -> stmt
-| s_while: expr bool -> stmt -> stmt
-| s_call: forall (pt : Type) rt, var rt -> proc pt rt -> expr pt -> stmt
+| s_if: expr t_bool -> stmt -> stmt -> stmt
+| s_while: expr t_bool -> stmt -> stmt
+| s_call: forall (pt : type) rt, var rt -> proc pt rt -> expr pt -> stmt
 | s_local: forall t, var t -> expr t -> stmt
 | s_return: forall t, expr t -> stmt
 | s_getlock: forall t, lock t -> stmt
@@ -66,7 +82,7 @@ with
 (*
  * procs both take and produce values
  *)
-(*Inductive*) proc: Type -> Type -> Type :=
+(*Inductive*) proc: type -> type -> Type :=
 | mkproc: forall pt rt, var pt -> stmt -> proc pt rt
 .
 
@@ -75,9 +91,14 @@ with
  * Extended/sugary AST forms
  *)
 
-Definition e_coqcall {ta tr : Set} (f : ta -> tr) (x : ta): expr tr :=
+Definition v_true: value t_bool := v_bool true.
+Definition v_false: value t_bool := v_bool false.
+
+(* doesn't quite work any more
+Definition e_coqcall {ta tr : type} (f : ta -> tr) (x : ta): expr tr :=
    e_value tr (f x)
 .
+*)
 
 Definition s_skip: stmt := s_block nil.
 
